common/Memory.v
@@ -43,6 +43,22 @@ Require Export Memtype.
 Local Unset Elimination Schemes.
 Local Unset Case Analysis Schemes.
 
+Instance inject_perm_upto_writable: InjectPerm :=
+  {
+    inject_perm_condition := fun p => perm_order Writable p
+  }.
+Proof.
+  tauto.
+Defined.
+
+Instance inject_perm_all: InjectPerm :=
+  {
+    inject_perm_condition := fun p => True
+  }.
+Proof.
+  tauto.
+Defined.
+
 Hint Resolve
   Mem.valid_not_valid_diff
   Mem.perm_implies
